WIP injection combinator
After help by talking with CJ, I found a bug in the statement of
[add_component]:

I think the statement of [add_component] is wrong; I think we don't need
[BtoA] nor [Htos], and instead want [mutators_match : forall idx m x m',
MutatorMethodSpecs B (Ms idx) (AtoB m) x m' -> exists m'', AtoB m'' =
m'].  (Alternatively, [m' = BtoA m' m''] in [mutators_match].)  I think
I'll be able to get this to work later tonight or tomorrow, though if
you want to look at the code again (I haven't changed anything) and tell
me if I'm wrong about [m' = AtoB m m''] being wrong, feel free.  (My
example is: A is (x, y); B is y; the mutator on A is (+1, +1); the
mutator on B is +1.)

Also, [add_component] ruled out non-deterministic mutators.

InternalADT.v
@@ -301,6 +301,63 @@ Section prod.
   Defined.
 End prod.
 
+(** A transformation (approximately, injection) from one ADT to another *)
+
+Section inj.
+  Variables A B : ADT.
+  (** Let's compose these two ADTs. *)
+
+  Variable BtoA : Model B -> Model A.
+  Variable mutatorMap : MutatorIndex B -> MutatorIndex A.
+  Variable observerMap : ObserverIndex B -> ObserverIndex A.
+  Hypothesis mutatorSpecMap
+  : forall idx m x m',
+      MutatorMethodSpecs A (mutatorMap idx) (BtoA m) x m'
+      -> exists m'',
+           m' = BtoA m''
+           /\ MutatorMethodSpecs B idx m x m''.
+  Hypothesis observerSpecMap
+  : forall idx m x y,
+      ObserverMethodSpecs A (observerMap idx) (BtoA m) x y
+      -> ObserverMethodSpecs B idx m x y.
+
+  Variable Ai : ADTimpl A.
+
+  Definition injImpl : ADTimpl B.
+  Proof.
+    refine {|
+        State := State Ai;
+        RepInv := fun (m : Model B) s
+                  => RepInv Ai (BtoA m) s;
+        MutatorMethodBodies name := MutatorMethodBodies Ai (mutatorMap name);
+        ObserverMethodBodies name := ObserverMethodBodies Ai (observerMap name)
+      |};
+    intro idx;
+    let H := fresh in
+    first [ assert (H := MutatorMethodsCorrect Ai (mutatorMap idx))
+          | assert (H := ObserverMethodsCorrect Ai (observerMap idx)) ];
+      let inv := fresh in
+      let x := fresh in
+      intros ? ? inv x;
+        specialize (H _ _ inv x);
+        simpl in *;
+        intuition;
+        let m := fresh "m" in
+        destruct H as [m H];
+          split_and.
+    let H0 := match goal with
+                | [ H : _ |- _ ] => constr:(@mutatorSpecMap _ _ _ _ H)
+              end in
+    let m := fresh "m" in
+    destruct H0 as [m ?];
+      split_and;
+      exists m;
+      subst;
+      intuition.
+   Defined.
+End inj.
+
+
 (** * An example, composing binary commutative associative calculators for computable nat multisets *)
 
 Definition multiset := nat -> nat.
@@ -838,6 +895,67 @@ Section prodPartial.
 End prodPartial.
 
 
+(** A transformation (approximately, injection) from one ADT to another *)
+
+Section injPartial.
+  Variables A B : ADT.
+  (** Let's compose these two ADTs. *)
+
+  Variable AtoB : Model A -> Model B.
+  Variable BtoA : Model B -> Model A.
+  Variable mutatorMap : MutatorIndex B -> MutatorIndex A.
+  Variable observerMap : ObserverIndex B -> ObserverIndex A.
+  Hypothesis mutatorSpecMap
+  : forall idx m x m',
+      MutatorMethodSpecs A (mutatorMap idx) (BtoA m) x m'
+      -> exists m'',
+           m' = BtoA m''
+           /\ MutatorMethodSpecs B idx m x m''.
+  Hypothesis observerSpecMap
+  : forall idx m x y,
+      ObserverMethodSpecs A (observerMap idx) (BtoA m) x y
+      -> ObserverMethodSpecs B idx m x y.
+
+
+  Variable Ai : PartialADTimpl A.
+
+  Definition injPartialImpl : PartialADTimpl B.
+  Proof.
+    refine {|
+        PState := PState Ai;
+        PRepInv := fun (m : Model B) s
+                  => PRepInv Ai (BtoA m) s;
+        PMutatorMethodBodies name := PMutatorMethodBodies Ai (mutatorMap name);
+        PObserverMethodBodies name := PObserverMethodBodies Ai (observerMap name)
+      |};
+    intro idx;
+    let H := fresh in
+    first [ assert (H := PMutatorMethodsCorrect Ai (mutatorMap idx))
+          | assert (H := PObserverMethodsCorrect Ai (observerMap idx));
+            edestruct PObserverMethodBodies; trivial ];
+      let inv := fresh in
+      let x := fresh in
+      intros ? ? inv x;
+        specialize (H _ _ inv x);
+        simpl in *;
+        intuition;
+        let m := fresh "m" in
+        destruct H as [m H];
+          split_and.
+    let H0 := match goal with
+                | [ H : _ |- _ ] => constr:(@mutatorSpecMap _ _ _ _ H)
+              end in
+    let m := fresh "m" in
+    destruct H0 as [m ?];
+      split_and;
+      exists m;
+      subst;
+      intuition.
+  Defined.
+End injPartial.
+
+
+(** Notes: it should be m' = BtoA m' m'' in mutators_match; actually we probably want [mutators_match : forall idx m x m', MutatorMethodSpecs B (Ms idx) (AtoB m) x m' -> exists m'', AtoB m'' = m'] *)
 Lemma add_component A B (Bimpl : ADTimpl B) later
   (Is : ObserverIndex A -> ObserverIndex B + later)
   (unlater : later -> ObserverIndex A)
@@ -846,10 +964,10 @@ Lemma add_component A B (Bimpl : ADTimpl B) later
   (BtoA : Model A -> Model B -> Model A)
   (Htos : forall m m', AtoB (BtoA m m') = m')
   (mutators_match : forall idx,
-    forall m x m' m'',
-      MutatorMethodSpecs A idx m x m'
-      -> MutatorMethodSpecs B (Ms idx) (AtoB m) x m''
-      -> m' = BtoA m m'')
+    forall m x m',
+      MutatorMethodSpecs B (Ms idx) (AtoB m) x m'
+      -> exists m'', m' = AtoB m''
+                     /\ MutatorMethodSpecs A idx m x m'')
   (observers_match : forall idx,
     match Is idx with
       | inr _ => True
@@ -868,6 +986,75 @@ Lemma add_component A B (Bimpl : ADTimpl B) later
   -> PartialADTimpl A.
 Proof.
   intro Aimpl.
+  pose (Bimpl : PartialADTimpl _) as Bimpl'.
+  Print Implicit injPartialImpl.
+  let A' := match type of Aimpl with PartialADTimpl ?A' => constr:(A') end in
+  pose (@pairedPartialImpl
+          A' B
+          (MutatorIndex A)
+          (ObserverIndex A)
+          (fun idx => (idx, Ms idx))
+          (fun idx => match Is idx with
+                        | inl idx' => inr idx'
+                        | inr idx' => inl idx'
+                      end)
+          Aimpl
+          Bimpl')
+    as ABimpl;
+    let AB := match type of ABimpl with PartialADTimpl ?AB => constr:(AB) end in
+    apply (fun g h =>
+            @injPartialImpl
+              AB A
+              (fun a => (a, AtoB a))
+              (fun x => x)
+              (fun x => x)
+              g h
+              ABimpl);
+    simpl in *;
+    try solve [ intuition ].
+  - intros idx m x [m'A m'B] ?; simpl in *.
+    intuition.
+    f_equal.
+    move mutators_match at bottom.
+
+    specialize (mutators_match _ _ _ _
+    esplit; intuition eauto.
+    move Htos at bottom.
+    move mutators_match at bottom.
+    erewrite (mutators_match _ m'A _ m'A) at 2; try eassumption.
+
+
+  - intros.
+    specialize (observers_match idx).
+    repeat match goal with
+             | [ H : appcontext[Is idx] |- _ ] => revert H
+           end.
+    case_eq (Is idx);
+      intros;
+      split_iff;
+      rewrite ?Htos' in *;
+      intuition.
+    erewrite <- almost_adjunction in * by eassumption; trivial.
+  - intros idx m x [m'A m'B] ?; simpl in *.
+    intuition.
+    f_equal.
+    move mutators_match at bottom.
+    specialize (
+    move Htos at bottom.
+    move mutators_match at bottom.
+    erewrite (mutators_match _ m'A _ m'A) at 2; try eassumption.
+
+
+
+    symmetry; eapply mutators_match; try eassumption.
+
+
+    rewrite <- (Htos m m0).
+
+    f_equal.
+
+
+ a). Aimpl Bimpl') as ABimpl.
   refine {|
     PState := PState Aimpl * State Bimpl;
     PRepInv := (fun (m : Model A) s
@@ -897,7 +1084,7 @@ Proof.
   intro idx;
     try (assert (MM := mutators_match idx));
       repeat intro;
-        simpl in *. 
+        simpl in *.
   split_and.
   edestruct (PMutatorMethodsCorrect Aimpl); try eassumption.
   edestruct (MutatorMethodsCorrect Bimpl); try eassumption.
@@ -989,7 +1176,7 @@ Goal PartialADTimpl NatSumProd_spec.
   exists (fun k => if eq_nat_dec x k then S (m k) else m k).
   auto.
 Defined.
-  
+
 
 Existing Class ADTimpl.
 Hint Extern 1 (ADTimpl _) => eapply NatLowerI : typeclass_instances.
